fixing #3049

ocaml/fstar-lib/generated/FStar_Tactics_Typeclasses.ml
@@ -485,7 +485,7 @@ let rec (mk_abs :
                                 (Prims.of_int (97)) (Prims.of_int (47)))))
                        (FStar_Sealed.seal
                           (Obj.magic
-                             (FStar_Range.mk_range "dummy" Prims.int_zero
+                             (FStar_Range.mk_range " dummy" Prims.int_zero
                                 Prims.int_zero Prims.int_zero Prims.int_zero)))
                        (Obj.magic
                           (FStar_Tactics_Effect.tac_bind
