src/typechecker/FStar.TypeChecker.Cfg.fst
@@ -542,8 +542,8 @@ let built_in_primitive_steps : prim_step_set =
         | _ -> failwith "Unexpected number of arguments"
     in
 
-    (* division is special cased since we must avoid zero denominators *)
-    let division_op : psc -> EMB.norm_cb -> universes -> args -> option term
+    (* division and modulus are special cased since we must avoid zero denominators *)
+    let division_modulus_op op : psc -> EMB.norm_cb -> universes -> args -> option term
       = fun psc _norm_cb _us args ->
         match args with
         | [(a1, None); (a2, None)] ->
@@ -551,13 +551,14 @@ let built_in_primitive_steps : prim_step_set =
                         try_unembed_simple EMB.e_int a2 with
             | Some m, Some n ->
               if Z.to_int_fs n <> 0
-              then Some (embed_simple EMB.e_int psc.psc_range (Z.div_big_int m n))
+              then Some (embed_simple EMB.e_int psc.psc_range (op m n))
               else None
 
             | _ -> None
             end
         | _ -> failwith "Unexpected number of arguments"
     in
+
     let bogus_cbs = {
         NBE.iapp = (fun h _args -> h);
         NBE.translate = (fun _ -> failwith "bogus_cbs translate");
@@ -607,8 +608,8 @@ let built_in_primitive_steps : prim_step_set =
          (PC.op_Division,
              2,
              0,
-             division_op,
-             (fun _us -> NBETerm.division_op));
+             division_modulus_op Z.div_big_int,
+             (fun _us -> NBETerm.division_modulus_op Z.div_big_int));
          (PC.op_LT,
              2,
              0,
@@ -632,8 +633,8 @@ let built_in_primitive_steps : prim_step_set =
          (PC.op_Modulus,
              2,
              0,
-             binary_int_op (fun x y -> Z.mod_big_int x y),
-             NBETerm.binary_int_op (fun x y -> Z.mod_big_int x y));
+             division_modulus_op Z.mod_big_int,
+             (fun _us -> NBETerm.division_modulus_op Z.mod_big_int));
          (PC.op_Negation,
              1,
              0,
