src/typechecker/FStar.TypeChecker.NBETerm.fsti
@@ -363,6 +363,6 @@ val dummy_interp : Ident.lid -> args -> option t
 val prims_to_fstar_range_step : args -> option t
 
 val mk_range : args -> option t
-val division_op : args -> option t
+val division_modulus_op (op:Z.bigint -> Z.bigint -> Z.bigint) : args -> option t
 val and_op : args -> option t
 val or_op : args -> option t
